let/Ariola.v
@@ -22,183 +22,183 @@ Inductive answer : term -> Prop :=
       answer a ->
       answer (Let t a).
 
-Inductive demands : var -> term -> Prop :=
-  | Demands_var x : demands x (Var x)
-  | Demands_appL t1 t2 x :
-      demands x t1 ->
-      demands x (App t1 t2)
-  | Demands_letL t1 t2 x :
-      demands x t1 ->
-      demands 0 t2 ->
-      demands x (Let t1 t2)
-  | Demands_letR t1 t2 x :
-      demands (S x) t2 ->
-      demands x (Let t1 t2).
+Inductive needs : term -> var -> Prop :=
+  | Needs_var x : needs (Var x) x
+  | Needs_appL t1 t2 x :
+      needs t1 x ->
+      needs (App t1 t2) x
+  | Needs_letL t1 t2 x :
+      needs t1 x ->
+      needs t2 0 ->
+      needs (Let t1 t2) x
+  | Needs_letR t1 t2 x :
+      needs t2 (S x) ->
+      needs (Let t1 t2) x.
 
-Inductive reassoc : term -> term -> Prop :=
-  | Reassoc_V v1 t2 t2' :
+Inductive reduceVCA : term -> term -> Prop :=
+  | ReduceVCA_V v1 t2 t2' :
       value v1 ->
-      demands 0 t2 ->
+      needs t2 0 ->
       t2' = t2.[v1/] ->
-      reassoc (Let v1 t2) t2'
-  | Reassoc_C t1 a2 t3 t3' :
+      reduceVCA (Let v1 t2) t2'
+  | ReduceVCA_C t1 a2 t3 t3' :
       answer a2 ->
       t3' = rename (+1)t3 ->
-      reassoc (App (Let t1 a2) t3) (Let t1 (App a2 t3'))
-  | Reassoc_A t1 a2 t3 t3' :
+      reduceVCA (App (Let t1 a2) t3) (Let t1 (App a2 t3'))
+  | ReduceVCA_A t1 a2 t3 t3' :
       answer a2 ->
-      demands 0 t3 ->
+      needs t3 0 ->
       t3' = rename (upren (+1)) t3 ->
-      reassoc (Let (Let t1 a2) t3) (Let t1 (Let a2 t3'))
-  | Reassoc_appL t1 t1' t2 :
-      reassoc t1 t1' ->
-      reassoc (App t1 t2) (App t1' t2)
-  | Reassoc_letL t1 t1' t2 :
-      reassoc t1 t1' ->
-      demands 0 t2 ->
-      reassoc (Let t1 t2) (Let t1' t2)
-  | Reassoc_letR t1 t2 t2' :
-      reassoc t2 t2' ->
-      reassoc (Let t1 t2) (Let t1 t2').
+      reduceVCA (Let (Let t1 a2) t3) (Let t1 (Let a2 t3'))
+  | ReduceVCA_appL t1 t1' t2 :
+      reduceVCA t1 t1' ->
+      reduceVCA (App t1 t2) (App t1' t2)
+  | ReduceVCA_letL t1 t1' t2 :
+      reduceVCA t1 t1' ->
+      needs t2 0 ->
+      reduceVCA (Let t1 t2) (Let t1' t2)
+  | ReduceVCA_letR t1 t2 t2' :
+      reduceVCA t2 t2' ->
+      reduceVCA (Let t1 t2) (Let t1 t2').
 
-Inductive red_need : term -> term -> Prop :=
+Inductive reduceI : term -> term -> Prop :=
   | RedNeed_I t1 t2 :
-      red_need (App (Lam t1) t2) (Let t2 t1)
+      reduceI (App (Lam t1) t2) (Let t2 t1)
   | RedNeed_appL t1 t1' t2 :
-      red_need t1 t1' ->
-      red_need (App t1 t2) (App t1' t2)
+      reduceI t1 t1' ->
+      reduceI (App t1 t2) (App t1' t2)
   | RedNeed_letL t1 t1' t2 :
-      red_need t1 t1' ->
-      demands 0 t2 ->
-      red_need (Let t1 t2) (Let t1' t2)
+      reduceI t1 t1' ->
+      needs t2 0 ->
+      reduceI (Let t1 t2) (Let t1' t2)
   | RedNeed_letR t1 t2 t2' :
-      red_need  t2 t2' ->
-      red_need (Let t1 t2) (Let t1 t2').
+      reduceI  t2 t2' ->
+      reduceI (Let t1 t2) (Let t1 t2').
 
-Hint Constructors value answer demands reassoc red_need clos_refl_trans.
+Hint Constructors value answer needs reduceVCA reduceI clos_refl_trans.
 
-Lemma reassoc_letL_multi t1 t1' t2 :
-  demands 0 t2 ->
-  clos_refl_trans _ reassoc t1 t1' ->
-  clos_refl_trans _ reassoc (Let t1 t2) (Let t1' t2).
+Lemma reduceVCA_letL_multi t1 t1' t2 :
+  needs t2 0 ->
+  clos_refl_trans _ reduceVCA t1 t1' ->
+  clos_refl_trans _ reduceVCA (Let t1 t2) (Let t1' t2).
 Proof. induction 2; eauto. Qed.
 
-Lemma reassoc_letR_multi t1 t2 t2' :
-  clos_refl_trans _ reassoc t2 t2' ->
-  clos_refl_trans _ reassoc (Let t1 t2) (Let t1 t2').
+Lemma reduceVCA_letR_multi t1 t2 t2' :
+  clos_refl_trans _ reduceVCA t2 t2' ->
+  clos_refl_trans _ reduceVCA (Let t1 t2) (Let t1 t2').
 Proof. induction 1; eauto. Qed.
 
-Hint Resolve reassoc_letL_multi reassoc_letR_multi.
+Hint Resolve reduceVCA_letL_multi reduceVCA_letR_multi.
 
 Section CallByNeedDeterminism.
   Lemma value_impl_answer v : value v -> answer v.
   Proof. inversion 1. constructor. Qed.
   Hint Resolve value_impl_answer.
 
-  Lemma answer_demands_disjoint a :
+  Lemma answer_needs_disjoint a :
     answer a ->
     forall x,
-    demands x a ->
+    needs a x ->
     False.
   Proof. induction 1; inversion 1; subst; eauto. Qed.
-  Hint Resolve answer_demands_disjoint.
+  Hint Resolve answer_needs_disjoint.
 
-  Lemma answer_reassoc_disjoint a :
+  Lemma answer_reduceVCA_disjoint a :
     answer a ->
     forall t,
-    reassoc a t ->
+    reduceVCA a t ->
     False.
   Proof. induction 1; inversion 1; subst; eauto. Qed.
 
-  Lemma answer_red_need_disjoint a :
+  Lemma answer_reduceI_disjoint a :
     answer a ->
     forall t,
-    red_need a t ->
+    reduceI a t ->
     False.
   Proof. induction 1; inversion 1; subst; eauto. Qed.
 
-  Lemma demands_unique x t :
-    demands x t ->
+  Lemma needs_unique x t :
+    needs t x ->
     forall y,
-    demands y t ->
+    needs t y ->
     x = y.
   Proof.
     induction 1; inversion 1; subst;
       repeat match goal with
-      | H : demands _ ?t, IH : forall x, demands x ?t -> _ = x |- _ => apply IH in H
+      | H : needs ?t _, IH : forall x, needs ?t x -> _ = x |- _ => apply IH in H
       end; congruence.
   Qed.
 
-  Lemma demands_reassoc_disjoint x t :
-    demands x t ->
+  Lemma needs_reduceVCA_disjoint t x :
+    needs t x ->
     forall t',
-    reassoc t t' ->
+    reduceVCA t t' ->
     False.
   Proof.
     induction 1; inversion 1; subst;
       repeat match goal with
-      | H : demands 0 ?t, H' : demands (S _) ?t |- _ => apply (demands_unique _ _ H) in H'; congruence
+      | H : needs ?t 0, H' : needs ?t (S _) |- _ => apply (needs_unique _ _ H) in H'; congruence
       end; eauto.
   Qed.
 
-  Lemma demands_red_need_disjoint x t :
-    demands x t ->
+  Lemma needs_reduceI_disjoint t x :
+    needs t x ->
     forall t',
-    red_need t t' ->
+    reduceI t t' ->
     False.
   Proof.
     induction 1; inversion 1; subst;
       repeat match goal with
-      | H : demands 0 ?t, H' : demands (S _) ?t |- _ => apply (demands_unique _ _ H) in H'; congruence
+      | H : needs ?t 0, H' : needs ?t (S _) |- _ => apply (needs_unique _ _ H) in H'; congruence
       end; eauto.
   Qed.
 
-  Lemma reassoc_red_need_disjoint t t' :
-    reassoc t t' ->
+  Lemma reduceVCA_reduceI_disjoint t t' :
+    reduceVCA t t' ->
     forall t'',
-    red_need t t'' ->
+    reduceI t t'' ->
     False.
   Proof.
-    Local Hint Resolve answer_red_need_disjoint demands_red_need_disjoint demands_reassoc_disjoint.
+    Local Hint Resolve answer_reduceI_disjoint needs_reduceI_disjoint needs_reduceVCA_disjoint.
     induction 1; inversion 1; subst; eauto.
     - inversion H.
   Qed.
 
-  Lemma reassoc_unique t t' :
-    reassoc t t' ->
+  Lemma reduceVCA_unique t t' :
+    reduceVCA t t' ->
     forall t'',
-    reassoc t t'' ->
+    reduceVCA t t'' ->
     t' = t''.
   Proof.
     induction 1; inversion 1; subst; f_equal;
       repeat match goal with
       | H : value (Let _ _) |- _ => inversion H
-      | H : reassoc ?t _ |- _ =>
+      | H : reduceVCA ?t _ |- _ =>
           let H' := fresh in
           assert (H' : answer t) by eauto;
-          destruct (answer_reassoc_disjoint _ H' _ H)
-      | H : demands _ ?t, H' : reassoc ?t _ |- _ => destruct (demands_reassoc_disjoint _ _ H _ H')
+          destruct (answer_reduceVCA_disjoint _ H' _ H)
+      | H : needs ?t _, H' : reduceVCA ?t _ |- _ => destruct (needs_reduceVCA_disjoint _ _ H _ H')
       end; eauto.
   Qed.
 
-  Lemma red_need_unique t t' :
-    red_need t t' ->
+  Lemma reduceI_unique t t' :
+    reduceI t t' ->
     forall t'',
-    red_need t t'' ->
+    reduceI t t'' ->
     t' = t''.
   Proof.
     induction 1; inversion 1; subst; f_equal;
       repeat match goal with
-      | H : red_need (Lam _) _ |- _ => inversion H
-      | H : demands _ ?t, H' : red_need ?t _ |- _ => destruct (demands_red_need_disjoint _ _ H _ H')
+      | H : reduceI (Lam _) _ |- _ => inversion H
+      | H : needs ?t _, H' : reduceI ?t _ |- _ => destruct (needs_reduceI_disjoint _ _ H _ H')
       end; eauto.
   Qed.
   
-  Theorem answer_or_reducible_or_stuck t :
+  Theorem answer_or_stuck_or_reducible t :
     answer t \/
-    (exists x, demands x t) \/
-    (exists t', reassoc t t') \/
-    (exists t', red_need t t').
+    (exists x, needs t x) \/
+    (exists t', reduceVCA t t') \/
+    (exists t', reduceI t t').
   Proof.
     induction t as
       [ | ? [ Hanswer | [ [ ] | [ [ ] | [ ] ] ] ]
@@ -207,7 +207,7 @@ Section CallByNeedDeterminism.
   Qed.
 End CallByNeedDeterminism.
 
-Section ReassocTerminating.
+Section ReduceVCATerminating.
   Fixpoint weight env t :=
     match t with
     | Var x => env x
@@ -290,8 +290,8 @@ Section ReassocTerminating.
       apply weight_rename.
   Qed.
 
-  Lemma weight_demands x t :
-    demands x t ->
+  Lemma weight_needs x t :
+    needs t x ->
     forall env env',
     (forall x, env x <= env' x) ->
     env x < env' x ->
@@ -301,18 +301,18 @@ Section ReassocTerminating.
     induction 1; simpl; intros ? ? Henv ?;
       repeat (rewrite plusnO || rewrite <- plus_assoc);
       repeat match goal with
-      | Hd : demands ?x ?t, He : ?env ?x < ?env' ?x |- weight ?env ?t + _ < weight ?env' ?t + _ => apply plus_lt_le_compat
+      | Hd : needs ?t ?x, He : ?env ?x < ?env' ?x |- weight ?env ?t + _ < weight ?env' ?t + _ => apply plus_lt_le_compat
       | |- _ + _ < _ + _ => apply plus_le_lt_compat
       | |- _ + _ <= _ + _ => apply plus_le_compat
       end; eauto.
     - apply weight_monotone.
-      intros [|?]; simpl; eauto.
-    - apply IHdemands; simpl; eauto.
-      intros [|?]; simpl; eauto.
+      intros [ | ? ]; simpl; eauto.
+    - apply IHneeds; simpl; eauto.
+      intros [ | ? ]; simpl; eauto.
   Qed.
 
-  Lemma reassoc_well_founded_aux t t' :
-    reassoc t t' ->
+  Lemma reduceVCA_well_founded_aux t t' :
+    reduceVCA t t' ->
     forall env, (forall x, 0 < env x) -> weight env t' < weight env t.
   Proof.
     induction 1; simpl; subst; intros env Henv;
@@ -320,7 +320,7 @@ Section ReassocTerminating.
     - rewrite weight_subst.
       rewrite plus_comm.
       apply lt_plus_trans.
-      apply (weight_demands _ _ H0); simpl.
+      apply (weight_needs _ _ H0); simpl.
       + intros [|?]; simpl; omega.
       + omega.
     - generalize (weight_least t1 _ Henv). intros ?.
@@ -331,29 +331,29 @@ Section ReassocTerminating.
       { apply weight_monotone.
         intros [|?]; simpl; omega. }
       omega.
-    - specialize (IHreassoc _ Henv).
+    - specialize (IHreduceVCA _ Henv).
       omega.
-    - generalize (IHreassoc _ Henv). intros ?.
+    - generalize (IHreduceVCA _ Henv). intros ?.
       apply plus_lt_le_compat.
       + omega.
       + apply weight_monotone.
         intros [|?]; simpl; omega.
     - apply plus_lt_compat_l.
-      apply IHreassoc.
+      apply IHreduceVCA.
       intros [|?]; simpl; eauto.
       omega.
   Qed.
 
-  Theorem reassoc_well_founded : well_founded (fun t t' => reassoc t' t).
+  Theorem reduceVCA_well_founded : well_founded (fun t t' => reduceVCA t' t).
   Proof.
     intros t.
     induction t as [ ? IH ] using (well_founded_induction (well_founded_ltof _ (weight (fun _ => 1)))).
     constructor.
-    intros ? Hreassoc.
+    intros ? HreduceVCA.
     apply IH.
-    apply reassoc_well_founded_aux; eauto.
+    apply reduceVCA_well_founded_aux; eauto.
   Qed.
-End ReassocTerminating.
+End ReduceVCATerminating.
 
 Section CallByNeedCorrectness.
   Fixpoint expand_let t :=
@@ -399,7 +399,7 @@ Section CallByNeedCorrectness.
     autosubst.
   Qed.
 
-  Lemma expand_let_reassoc t t' : reassoc t t' -> expand_let t = expand_let t'.
+  Lemma expand_let_reduceVCA t t' : reduceVCA t t' -> expand_let t = expand_let t'.
   Proof.
     induction 1; subst; simpl;
       try solve [ repeat rewrite <- expand_let_subst_single; repeat (f_equal; autosubst) ];
@@ -414,17 +414,17 @@ Section CallByNeedCorrectness.
     rewrite IHanswer. simpl. eauto.
   Qed.
 
-  Lemma expand_let_demands x t :
-    demands x t ->
-    stuck_in_var x (expand_let t).
+  Lemma expand_let_needs x t :
+    needs t x ->
+    needsn (expand_let t) x.
   Proof.
     induction 1; simpl; eauto.
-    - eapply stuck_in_var_subst; eauto.
-    - apply stuck_in_var_subst with (x := S x); simpl; eauto.
+    - eapply needsn_subst; eauto.
+    - apply needsn_subst with (x := S x); simpl; eauto.
   Qed.
 
-  Lemma expand_let_red_need t t' :
-    red_need t t' ->
+  Lemma expand_let_reduceI t t' :
+    reduceI t t' ->
     exists t0, cbn (expand_let t) t0 /\ clos_refl_trans _ red t0 (expand_let t').
   Proof.
     induction 1 as
@@ -433,25 +433,25 @@ Section CallByNeedCorrectness.
         | ? ? ? ? [ ? [ ] ] ]; simpl; eauto.
     - eapply cbn_subst' with (x := 0); simpl; eauto.
       + intros [ ]; eauto.
-      + apply expand_let_demands; eauto.
+      + apply expand_let_needs; eauto.
     - eexists.  split.
       + apply cbn_subst. eauto.
       + eapply red_subst_multi; eauto.
   Qed.
 
   Lemma red_need_sound_aux t t' :
-    clos_refl_trans _ (fun t t' => reassoc t t' \/ red_need t t') t t' ->
+    clos_refl_trans _ (fun t t' => reduceVCA t t' \/ reduceI t t') t t' ->
     clos_refl_trans _ red (expand_let t) (expand_let t').
   Proof.
     intros Hrt.
     apply clos_rt_rt1n in Hrt.
-    induction Hrt as [ | ? ? ? [ Hreassoc | Hred ] ]; eauto.
-    - apply expand_let_reassoc in Hreassoc. congruence.
-    - destruct (expand_let_red_need _ _ Hred) as [ ? [ ] ]. eauto.
+    induction Hrt as [ | ? ? ? [ HreduceVCA | Hred ] ]; eauto.
+    - apply expand_let_reduceVCA in HreduceVCA. congruence.
+    - destruct (expand_let_reduceI _ _ Hred) as [ ? [ ] ]. eauto.
   Qed.
 
   Theorem red_need_sound t t' :
-    clos_refl_trans _ (fun t t' => reassoc t t' \/ red_need t t') t t' ->
+    clos_refl_trans _ (fun t t' => reduceVCA t t' \/ reduceI t t') t t' ->
     answer t' ->
     exists t0, clos_refl_trans _ cbn (expand_let t) (tabs t0) /\ clos_refl_trans _ red (tabs t0) (expand_let t').
   Proof.
@@ -468,28 +468,28 @@ Section CallByNeedCorrectness.
   Lemma red_need_normalize t0 :
     Acc (fun t3 t1 => exists t2, cbn t1 t2 /\ clos_refl_trans _ red t2 t3) t0 ->
     forall t, expand_let t = t0 ->
-    exists t', clos_refl_trans _ (fun t t' => reassoc t t' \/ red_need t t') t t' /\ in_normal_form _ (fun t t' => reassoc t t' \/ red_need t t') t'.
+    exists t', clos_refl_trans _ (fun t t' => reduceVCA t t' \/ reduceI t t') t t' /\ in_normal_form _ (fun t t' => reduceVCA t t' \/ reduceI t t') t'.
   Proof.
     induction 1 as [ ? ? IH ]. intros t ?. subst.
-    induction t as [ ? IH' ] using (well_founded_induction reassoc_well_founded).
-    destruct (answer_or_reducible_or_stuck t) as [ ? | [ [ ? ? ] | [ [ ? Hreassoc ] | [ ? Hred ] ] ] ]; eauto.
+    induction t as [ ? IH' ] using (well_founded_induction reduceVCA_well_founded).
+    destruct (answer_or_stuck_or_reducible t) as [ ? | [ [ ? ? ] | [ [ ? HreduceVCA ] | [ ? Hred ] ] ] ]; eauto.
     - exists t. split; eauto.
       intros ? [ ? | ? ].
-      + eapply answer_reassoc_disjoint; eauto.
-      + eapply answer_red_need_disjoint; eauto.
+      + eapply answer_reduceVCA_disjoint; eauto.
+      + eapply answer_reduceI_disjoint; eauto.
     - exists t. split; eauto.
       intros ? [ ? | ? ].
-      + eapply demands_reassoc_disjoint; eauto.
-      + eapply demands_red_need_disjoint; eauto.
-    - destruct (IH' _ Hreassoc) as [ ? [ ] ];
-        try rewrite <- (expand_let_reassoc _ _ Hreassoc) in *;
+      + eapply needs_reduceVCA_disjoint; eauto.
+      + eapply needs_reduceI_disjoint; eauto.
+    - destruct (IH' _ HreduceVCA) as [ ? [ ] ];
+        try rewrite <- (expand_let_reduceVCA _ _ HreduceVCA) in *;
         eauto 6.
-    - destruct (IH _ (expand_let_red_need _ _ Hred) _ eq_refl) as [ ? [ ] ]. eauto 6.
+    - destruct (IH _ (expand_let_reduceI _ _ Hred) _ eq_refl) as [ ? [ ] ]. eauto 6.
   Qed.
 
   Theorem red_need_complete t t0 :
     clos_refl_trans _ cbn (expand_let t) (tabs t0) ->
-    exists t', clos_refl_trans _ (fun t t' => reassoc t t' \/ red_need t t') t t' /\ answer t' /\ clos_refl_trans _ red (tabs t0) (expand_let t').
+    exists t', clos_refl_trans _ (fun t t' => reduceVCA t t' \/ reduceI t t') t t' /\ answer t' /\ clos_refl_trans _ red (tabs t0) (expand_let t').
   Proof.
     intros Hnormalizing.
     edestruct red_need_normalize with (t := t) as [ t' [ Hrt Hnf ] ]; eauto.
@@ -497,7 +497,7 @@ Section CallByNeedCorrectness.
       eapply normalizing_and_deterministic_impl_terminating; eauto.
       + intros ? ? ? ?. apply cbn_det; eauto.
       + inversion 1.
-    - destruct (answer_or_reducible_or_stuck t') as [ Hanswer | [ [ ? Hdemands ] | [ [ ? Hreassoc ] | [ ? Hred ] ] ] ].
+    - destruct (answer_or_stuck_or_reducible t') as [ Hanswer | [ [ ? Hneeds ] | [ [ ? HreduceVCA ] | [ ? Hred ] ] ] ].
       + destruct (red_need_sound _ _ Hrt Hanswer) as [ ? [ Hnormalizing' ] ].
         destruct (cbn_confluent _ _ _ Hnormalizing Hnormalizing') as [ ? [ Hrefl Hrefl' ] ].
         destruct (strip_lemma _ _ _ _ Hrefl) as [ | [ ? [ Hcontra ]] ]; [ subst | inversion Hcontra ].
@@ -505,7 +505,7 @@ Section CallByNeedCorrectness.
       + apply red_need_sound_aux in Hrt.
         destruct (red_confluent _ _ _ (cbn_multi_impl_red_multi _ _ Hnormalizing) Hrt) as [ ? [ Hrt' Hrt'' ] ].
         destruct (red_abs_multi_inv _ _ Hrt' _ eq_refl) as [? [ ] ]. subst.
-        specialize (stuck_in_var_preserved_by_red_multi _ _ _ Hrt'' (expand_let_demands _ _ Hdemands)).
+        specialize (needsn_preserved_by_red_multi _ _ _ Hrt'' (expand_let_needs _ _ Hneeds)).
         inversion 1.
       + edestruct Hnf; simpl; eauto.
       + edestruct Hnf; simpl; eauto.
